Show: Skolem terms stay valid when renaming consts

ExistentialRules/ChaseSequence/Termination/RenameConstantsApart.lean
@@ -29,6 +29,84 @@ mutual
 
 end
 
+mutual
+
+  theorem PreGroundTerm.rename_constants_apart_preserves_ruleId_validity [GetFreshRepresentant sig.C] (term : FiniteTree (SkolemFS sig) sig.C) (forbidden_constants : List sig.C) :
+      ∀ rl, PreGroundTerm.skolem_ruleIds_valid rl term -> PreGroundTerm.skolem_ruleIds_valid rl (PreGroundTerm.rename_constants_apart term forbidden_constants) := by
+    intro rl valid
+    cases term with
+    | leaf _ => simp [rename_constants_apart, skolem_ruleIds_valid]
+    | inner func ts =>
+      simp only [rename_constants_apart, skolem_ruleIds_valid] at *
+      constructor
+      . exact valid.left
+      . apply PreGroundTerm.rename_constants_apart_preserves_ruleId_validity_list; exact valid.right
+
+  theorem PreGroundTerm.rename_constants_apart_preserves_ruleId_validity_list [GetFreshRepresentant sig.C] (terms : FiniteTreeList (SkolemFS sig) sig.C) (forbidden_constants : List sig.C) :
+      ∀ rl, PreGroundTerm.skolem_ruleIds_valid_list rl terms -> PreGroundTerm.skolem_ruleIds_valid_list rl (PreGroundTerm.rename_constants_apart_list terms forbidden_constants) := by
+    intro rl valid
+    cases terms with
+    | nil => simp [rename_constants_apart_list, skolem_ruleIds_valid_list]
+    | cons hd tl =>
+      simp only [rename_constants_apart_list, skolem_ruleIds_valid_list] at *
+      constructor
+      . apply PreGroundTerm.rename_constants_apart_preserves_ruleId_validity; exact valid.left
+      . apply PreGroundTerm.rename_constants_apart_preserves_ruleId_validity_list; exact valid.right
+
+end
+
+mutual
+
+  theorem PreGroundTerm.rename_constants_apart_preserves_disjIdx_validity [GetFreshRepresentant sig.C] (term : FiniteTree (SkolemFS sig) sig.C) (forbidden_constants : List sig.C) :
+      ∀ rl, (h : PreGroundTerm.skolem_ruleIds_valid rl term) -> PreGroundTerm.skolem_disjIdx_valid rl term h -> PreGroundTerm.skolem_disjIdx_valid rl (PreGroundTerm.rename_constants_apart term forbidden_constants) (PreGroundTerm.rename_constants_apart_preserves_ruleId_validity term forbidden_constants rl h) := by
+    intro rl _ valid
+    cases term with
+    | leaf _ => simp [rename_constants_apart, skolem_disjIdx_valid]
+    | inner func ts =>
+      simp only [rename_constants_apart, skolem_disjIdx_valid] at *
+      constructor
+      . exact valid.left
+      . apply PreGroundTerm.rename_constants_apart_preserves_disjIdx_validity_list; exact valid.right
+
+  theorem PreGroundTerm.rename_constants_apart_preserves_disjIdx_validity_list [GetFreshRepresentant sig.C] (terms : FiniteTreeList (SkolemFS sig) sig.C) (forbidden_constants : List sig.C) :
+      ∀ rl, (h : PreGroundTerm.skolem_ruleIds_valid_list rl terms) -> PreGroundTerm.skolem_disjIdx_valid_list rl terms h -> PreGroundTerm.skolem_disjIdx_valid_list rl (PreGroundTerm.rename_constants_apart_list terms forbidden_constants) (PreGroundTerm.rename_constants_apart_preserves_ruleId_validity_list terms forbidden_constants rl h) := by
+    intro rl _ valid
+    cases terms with
+    | nil => simp [rename_constants_apart_list, skolem_disjIdx_valid_list]
+    | cons hd tl =>
+      simp only [rename_constants_apart_list, skolem_disjIdx_valid_list] at *
+      constructor
+      . apply PreGroundTerm.rename_constants_apart_preserves_disjIdx_validity; exact valid.left
+      . apply PreGroundTerm.rename_constants_apart_preserves_disjIdx_validity_list; exact valid.right
+
+end
+
+mutual
+
+  theorem PreGroundTerm.rename_constants_apart_preserves_rule_arity_validity [GetFreshRepresentant sig.C] (term : FiniteTree (SkolemFS sig) sig.C) (forbidden_constants : List sig.C) :
+      ∀ rl, (h : PreGroundTerm.skolem_ruleIds_valid rl term) -> PreGroundTerm.skolem_rule_arity_valid rl term h -> PreGroundTerm.skolem_rule_arity_valid rl (PreGroundTerm.rename_constants_apart term forbidden_constants) (PreGroundTerm.rename_constants_apart_preserves_ruleId_validity term forbidden_constants rl h) := by
+    intro rl _ valid
+    cases term with
+    | leaf _ => simp [rename_constants_apart, skolem_rule_arity_valid]
+    | inner func ts =>
+      simp only [rename_constants_apart, skolem_rule_arity_valid] at *
+      constructor
+      . exact valid.left
+      . apply PreGroundTerm.rename_constants_apart_preserves_rule_arity_validity_list; exact valid.right
+
+  theorem PreGroundTerm.rename_constants_apart_preserves_rule_arity_validity_list [GetFreshRepresentant sig.C] (terms : FiniteTreeList (SkolemFS sig) sig.C) (forbidden_constants : List sig.C) :
+      ∀ rl, (h : PreGroundTerm.skolem_ruleIds_valid_list rl terms) -> PreGroundTerm.skolem_rule_arity_valid_list rl terms h -> PreGroundTerm.skolem_rule_arity_valid_list rl (PreGroundTerm.rename_constants_apart_list terms forbidden_constants) (PreGroundTerm.rename_constants_apart_preserves_ruleId_validity_list terms forbidden_constants rl h) := by
+    intro rl _ valid
+    cases terms with
+    | nil => simp [rename_constants_apart_list, skolem_rule_arity_valid_list]
+    | cons hd tl =>
+      simp only [rename_constants_apart_list, skolem_rule_arity_valid_list] at *
+      constructor
+      . apply PreGroundTerm.rename_constants_apart_preserves_rule_arity_validity; exact valid.left
+      . apply PreGroundTerm.rename_constants_apart_preserves_rule_arity_validity_list; exact valid.right
+
+end
+
 def GroundTerm.rename_constants_apart
     [GetFreshRepresentant sig.C]
     (term : GroundTerm sig)
@@ -67,16 +145,36 @@ def GroundTerm.rename_constants_apart
         simp
   ⟩
 
+theorem GroundTerm.rename_constants_apart_preserves_ruleId_validity [GetFreshRepresentant sig.C] (term : GroundTerm sig) (forbidden_constants : List sig.C) :
+    ∀ rl, GroundTerm.skolem_ruleIds_valid rl term -> GroundTerm.skolem_ruleIds_valid rl (GroundTerm.rename_constants_apart term forbidden_constants) := by
+  intro rl valid
+  simp only [rename_constants_apart, skolem_ruleIds_valid] at *
+  apply PreGroundTerm.rename_constants_apart_preserves_ruleId_validity
+  exact valid
 
-def PreTrigger.rename_constants_apart [GetFreshRepresentant sig.C] (trg : PreTrigger sig) : PreTrigger sig :=
+theorem GroundTerm.rename_constants_apart_preserves_disjIdx_validity [GetFreshRepresentant sig.C] (term : GroundTerm sig) (forbidden_constants : List sig.C) :
+    ∀ rl, (h : GroundTerm.skolem_ruleIds_valid rl term) -> GroundTerm.skolem_disjIdx_valid rl term h -> GroundTerm.skolem_disjIdx_valid rl (GroundTerm.rename_constants_apart term forbidden_constants) (GroundTerm.rename_constants_apart_preserves_ruleId_validity term forbidden_constants rl h) := by
+  intro rl _ valid
+  simp only [rename_constants_apart, skolem_ruleIds_valid] at *
+  apply PreGroundTerm.rename_constants_apart_preserves_disjIdx_validity
+  exact valid
+
+theorem GroundTerm.rename_constants_apart_preserves_rule_arity_validity [GetFreshRepresentant sig.C] (term : GroundTerm sig) (forbidden_constants : List sig.C) :
+    ∀ rl, (h : GroundTerm.skolem_ruleIds_valid rl term) -> GroundTerm.skolem_rule_arity_valid rl term h -> GroundTerm.skolem_rule_arity_valid rl (GroundTerm.rename_constants_apart term forbidden_constants) (GroundTerm.rename_constants_apart_preserves_ruleId_validity term forbidden_constants rl h) := by
+  intro rl _ valid
+  simp only [rename_constants_apart, skolem_ruleIds_valid] at *
+  apply PreGroundTerm.rename_constants_apart_preserves_rule_arity_validity
+  exact valid
+
+def PreTrigger.rename_constants_apart [GetFreshRepresentant sig.C] (trg : PreTrigger sig) (forbidden_constants : List sig.C) : PreTrigger sig :=
   let renamed_apart_terms_for_body_vars : List (GroundTerm sig) := trg.rule.body.vars.foldl (fun acc v =>
-    let forbidden_constants := acc.flatMap GroundTerm.constants
-    acc ++ [(trg.subs v).rename_constants_apart forbidden_constants]
+    let forbidden_constants_inner := acc.flatMap GroundTerm.constants
+    acc ++ [(trg.subs v).rename_constants_apart (forbidden_constants ++ forbidden_constants_inner)]
   ) []
 
   have length_preserved : ∀ (l : List sig.V) (init : List (GroundTerm sig)), (l.foldl (fun acc v =>
-    let forbidden_constants := acc.flatMap GroundTerm.constants
-    acc ++ [(trg.subs v).rename_constants_apart forbidden_constants]
+    let forbidden_constants_inner := acc.flatMap GroundTerm.constants
+    acc ++ [(trg.subs v).rename_constants_apart (forbidden_constants ++ forbidden_constants_inner)]
   ) init).length = init.length + l.length := by
     intro l
     induction l with
@@ -98,4 +196,287 @@ def PreTrigger.rename_constants_apart [GetFreshRepresentant sig.C] (trg : PreTri
       renamed_apart_terms_for_body_vars[idx]
     else trg.subs x -- it should not matter what we return here
   ⟩
+
+-- TODO: the following three proofs seem way too complicated; maybe I'm too tired already to see how to simplify; or it's really that bad...
+theorem PreTrigger.rename_constants_apart_preserves_ruleId_validity [GetFreshRepresentant sig.C] (trg : PreTrigger sig) (forbidden_constants : List sig.C) :
+    ∀ rl, PreTrigger.skolem_ruleIds_valid rl trg -> PreTrigger.skolem_ruleIds_valid rl (PreTrigger.rename_constants_apart trg forbidden_constants) := by
+  intro rl valid
+  simp only [rename_constants_apart, skolem_ruleIds_valid] at *
+  intro t t_mem
+  rw [List.mem_flatMap] at t_mem
+  rcases t_mem with ⟨f, f_mem, t_mem⟩
+  simp only [PreTrigger.mapped_body, GroundSubstitution.apply_function_free_conj] at f_mem
+  rw [List.mem_map] at f_mem
+  simp only [GroundSubstitution.apply_function_free_atom] at f_mem
+  rcases f_mem with ⟨a, a_mem, f_eq⟩
+  rw [← f_eq] at t_mem
+  simp only at t_mem
+  rw [List.mem_map] at t_mem
+  rcases t_mem with ⟨voc, voc_mem, t_eq⟩
+  rw [← t_eq]
+  cases voc with
+  | const c =>
+    simp only [GroundSubstitution.apply_var_or_const]
+    apply GroundTerm.skolem_ruleIds_valid_const
+  | var v =>
+    have : v ∈ trg.rule.body.vars := by
+      unfold FunctionFreeConjunction.vars
+      rw [List.mem_flatMap]
+      exists a
+      constructor
+      . exact a_mem
+      . unfold FunctionFreeAtom.variables
+        apply VarOrConst.mem_filterVars_of_var
+        exact voc_mem
+    simp only [GroundSubstitution.apply_var_or_const, this, ↓reduceDIte]
+
+    have : ∀ (l : List sig.V) (subset : l ⊆ trg.rule.body.vars) (init : List (GroundTerm sig)) (init_valid : ∀ t ∈ init, t.skolem_ruleIds_valid rl) (t : GroundTerm sig), t ∈ (l.foldl (fun acc v =>
+      let forbidden_constants_inner := acc.flatMap GroundTerm.constants
+      acc ++ [(trg.subs v).rename_constants_apart (forbidden_constants ++ forbidden_constants_inner)]
+    ) init) -> t.skolem_ruleIds_valid rl := by
+      intro l
+      induction l with
+      | nil =>
+        intro _ init init_valid t t_mem
+        rw [List.foldl_nil] at t_mem
+        apply init_valid
+        exact t_mem
+      | cons hd tl ih =>
+        intro subset init init_valid t t_mem
+        rw [List.foldl_cons] at t_mem
+        apply ih _ _ _ t
+        . exact t_mem
+        . intro e e_mem; apply subset; simp [e_mem]
+        . intro t t_mem
+          rw [List.mem_append, List.mem_singleton] at t_mem
+          cases t_mem with
+          | inl t_mem => apply init_valid; exact t_mem
+          | inr t_mem =>
+            rw [t_mem]
+            apply GroundTerm.rename_constants_apart_preserves_ruleId_validity
+            apply valid
+            specialize subset List.mem_cons_self
+            unfold FunctionFreeConjunction.vars at subset
+            rw [List.mem_flatMap] at subset
+            rw [List.mem_flatMap]
+            rcases subset with ⟨a, a_mem, hd_mem⟩
+            exists trg.subs.apply_function_free_atom a
+            constructor
+            . apply List.mem_map_of_mem; exact a_mem
+            . simp only [GroundSubstitution.apply_function_free_atom]
+              unfold FunctionFreeAtom.variables at hd_mem
+              rw [List.mem_map]
+              exists VarOrConst.var hd
+              constructor
+              . apply VarOrConst.filterVars_occur_in_original_list; exact hd_mem
+              . simp [GroundSubstitution.apply_var_or_const]
+
+    apply this trg.rule.body.vars _ []
+    . apply List.getElem_mem
+    . simp
+    . simp
+
+theorem PreTrigger.rename_constants_apart_preserves_disjIdx_validity [GetFreshRepresentant sig.C] (trg : PreTrigger sig) (forbidden_constants : List sig.C) :
+    ∀ rl, (h : PreTrigger.skolem_ruleIds_valid rl trg) -> PreTrigger.skolem_disjIdx_valid rl trg h -> PreTrigger.skolem_disjIdx_valid rl (PreTrigger.rename_constants_apart trg forbidden_constants) (PreTrigger.rename_constants_apart_preserves_ruleId_validity trg forbidden_constants rl h) := by
+  intro rl h valid
+  simp only [rename_constants_apart, skolem_ruleIds_valid] at *
+  intro t t_mem
+  rw [List.mem_flatMap] at t_mem
+  rcases t_mem with ⟨f, f_mem, t_mem⟩
+  simp only [PreTrigger.mapped_body, GroundSubstitution.apply_function_free_conj] at f_mem
+  rw [List.mem_map] at f_mem
+  simp only [GroundSubstitution.apply_function_free_atom] at f_mem
+  rcases f_mem with ⟨a, a_mem, f_eq⟩
+  rw [← f_eq] at t_mem
+  simp only at t_mem
+  rw [List.mem_map] at t_mem
+  rcases t_mem with ⟨voc, voc_mem, t_eq⟩
+  simp only [← t_eq]
+  cases voc with
+  | const c =>
+    simp only [GroundSubstitution.apply_var_or_const]
+    apply GroundTerm.skolem_disjIdx_valid_const
+  | var v =>
+    have : v ∈ trg.rule.body.vars := by
+      unfold FunctionFreeConjunction.vars
+      rw [List.mem_flatMap]
+      exists a
+      constructor
+      . exact a_mem
+      . unfold FunctionFreeAtom.variables
+        apply VarOrConst.mem_filterVars_of_var
+        exact voc_mem
+    simp only [GroundSubstitution.apply_var_or_const, this, ↓reduceDIte]
+
+    have : ∀ (l : List sig.V) (subset : l ⊆ trg.rule.body.vars) (init : List (GroundTerm sig)) (init_h : ∀ t ∈ init, t.skolem_ruleIds_valid rl) (init_valid : ∀ t, (t_mem : t ∈ init) -> t.skolem_disjIdx_valid rl (init_h t t_mem)) (t : GroundTerm sig), (t_h : t.skolem_ruleIds_valid rl) -> t ∈ (l.foldl (fun acc v =>
+      let forbidden_constants_inner := acc.flatMap GroundTerm.constants
+      acc ++ [(trg.subs v).rename_constants_apart (forbidden_constants ++ forbidden_constants_inner)]
+    ) init) -> t.skolem_disjIdx_valid rl t_h := by
+      intro l
+      induction l with
+      | nil =>
+        intro _ init init_h init_valid t t_h t_mem
+        rw [List.foldl_nil] at t_mem
+        apply init_valid
+        exact t_mem
+      | cons hd tl ih =>
+        intro subset init init_h init_valid t t_h t_mem
+        rw [List.foldl_cons] at t_mem
+        apply ih _ _ _ _ t
+        . exact t_mem
+        . intro e e_mem; apply subset; simp [e_mem]
+        . intro t t_mem
+          rw [List.mem_append, List.mem_singleton] at t_mem
+          cases t_mem with
+          | inl t_mem => apply init_h; exact t_mem
+          | inr t_mem =>
+            simp only [t_mem]
+            apply GroundTerm.rename_constants_apart_preserves_ruleId_validity
+            apply h
+            specialize subset List.mem_cons_self
+            unfold FunctionFreeConjunction.vars at subset
+            rw [List.mem_flatMap] at subset
+            rw [List.mem_flatMap]
+            rcases subset with ⟨a, a_mem, hd_mem⟩
+            exists trg.subs.apply_function_free_atom a
+            constructor
+            . apply List.mem_map_of_mem; exact a_mem
+            . simp only [GroundSubstitution.apply_function_free_atom]
+              unfold FunctionFreeAtom.variables at hd_mem
+              rw [List.mem_map]
+              exists VarOrConst.var hd
+              constructor
+              . apply VarOrConst.filterVars_occur_in_original_list; exact hd_mem
+              . simp [GroundSubstitution.apply_var_or_const]
+        . intro t t_mem
+          rw [List.mem_append, List.mem_singleton] at t_mem
+          cases t_mem with
+          | inl t_mem => apply init_valid; exact t_mem
+          | inr t_mem =>
+            simp only [t_mem]
+            apply GroundTerm.rename_constants_apart_preserves_disjIdx_validity
+            apply valid
+            specialize subset List.mem_cons_self
+            unfold FunctionFreeConjunction.vars at subset
+            rw [List.mem_flatMap] at subset
+            rw [List.mem_flatMap]
+            rcases subset with ⟨a, a_mem, hd_mem⟩
+            exists trg.subs.apply_function_free_atom a
+            constructor
+            . apply List.mem_map_of_mem; exact a_mem
+            . simp only [GroundSubstitution.apply_function_free_atom]
+              unfold FunctionFreeAtom.variables at hd_mem
+              rw [List.mem_map]
+              exists VarOrConst.var hd
+              constructor
+              . apply VarOrConst.filterVars_occur_in_original_list; exact hd_mem
+              . simp [GroundSubstitution.apply_var_or_const]
+
+    apply this trg.rule.body.vars _ []
+    . apply List.getElem_mem
+    . simp
+    . simp
+    . simp
+
+theorem PreTrigger.rename_constants_apart_preserves_rule_arity_validity [GetFreshRepresentant sig.C] (trg : PreTrigger sig) (forbidden_constants : List sig.C) :
+    ∀ rl, (h : PreTrigger.skolem_ruleIds_valid rl trg) -> PreTrigger.skolem_rule_arity_valid rl trg h -> PreTrigger.skolem_rule_arity_valid rl (PreTrigger.rename_constants_apart trg forbidden_constants) (PreTrigger.rename_constants_apart_preserves_ruleId_validity trg forbidden_constants rl h) := by
+  intro rl h valid
+  simp only [rename_constants_apart, skolem_ruleIds_valid] at *
+  intro t t_mem
+  rw [List.mem_flatMap] at t_mem
+  rcases t_mem with ⟨f, f_mem, t_mem⟩
+  simp only [PreTrigger.mapped_body, GroundSubstitution.apply_function_free_conj] at f_mem
+  rw [List.mem_map] at f_mem
+  simp only [GroundSubstitution.apply_function_free_atom] at f_mem
+  rcases f_mem with ⟨a, a_mem, f_eq⟩
+  rw [← f_eq] at t_mem
+  simp only at t_mem
+  rw [List.mem_map] at t_mem
+  rcases t_mem with ⟨voc, voc_mem, t_eq⟩
+  simp only [← t_eq]
+  cases voc with
+  | const c =>
+    simp only [GroundSubstitution.apply_var_or_const]
+    apply GroundTerm.skolem_rule_arity_valid_const
+  | var v =>
+    have : v ∈ trg.rule.body.vars := by
+      unfold FunctionFreeConjunction.vars
+      rw [List.mem_flatMap]
+      exists a
+      constructor
+      . exact a_mem
+      . unfold FunctionFreeAtom.variables
+        apply VarOrConst.mem_filterVars_of_var
+        exact voc_mem
+    simp only [GroundSubstitution.apply_var_or_const, this, ↓reduceDIte]
+
+    have : ∀ (l : List sig.V) (subset : l ⊆ trg.rule.body.vars) (init : List (GroundTerm sig)) (init_h : ∀ t ∈ init, t.skolem_ruleIds_valid rl) (init_valid : ∀ t, (t_mem : t ∈ init) -> t.skolem_rule_arity_valid rl (init_h t t_mem)) (t : GroundTerm sig), (t_h : t.skolem_ruleIds_valid rl) -> t ∈ (l.foldl (fun acc v =>
+      let forbidden_constants_inner := acc.flatMap GroundTerm.constants
+      acc ++ [(trg.subs v).rename_constants_apart (forbidden_constants ++ forbidden_constants_inner)]
+    ) init) -> t.skolem_rule_arity_valid rl t_h := by
+      intro l
+      induction l with
+      | nil =>
+        intro _ init init_h init_valid t t_h t_mem
+        rw [List.foldl_nil] at t_mem
+        apply init_valid
+        exact t_mem
+      | cons hd tl ih =>
+        intro subset init init_h init_valid t t_h t_mem
+        rw [List.foldl_cons] at t_mem
+        apply ih _ _ _ _ t
+        . exact t_mem
+        . intro e e_mem; apply subset; simp [e_mem]
+        . intro t t_mem
+          rw [List.mem_append, List.mem_singleton] at t_mem
+          cases t_mem with
+          | inl t_mem => apply init_h; exact t_mem
+          | inr t_mem =>
+            simp only [t_mem]
+            apply GroundTerm.rename_constants_apart_preserves_ruleId_validity
+            apply h
+            specialize subset List.mem_cons_self
+            unfold FunctionFreeConjunction.vars at subset
+            rw [List.mem_flatMap] at subset
+            rw [List.mem_flatMap]
+            rcases subset with ⟨a, a_mem, hd_mem⟩
+            exists trg.subs.apply_function_free_atom a
+            constructor
+            . apply List.mem_map_of_mem; exact a_mem
+            . simp only [GroundSubstitution.apply_function_free_atom]
+              unfold FunctionFreeAtom.variables at hd_mem
+              rw [List.mem_map]
+              exists VarOrConst.var hd
+              constructor
+              . apply VarOrConst.filterVars_occur_in_original_list; exact hd_mem
+              . simp [GroundSubstitution.apply_var_or_const]
+        . intro t t_mem
+          rw [List.mem_append, List.mem_singleton] at t_mem
+          cases t_mem with
+          | inl t_mem => apply init_valid; exact t_mem
+          | inr t_mem =>
+            simp only [t_mem]
+            apply GroundTerm.rename_constants_apart_preserves_rule_arity_validity
+            apply valid
+            specialize subset List.mem_cons_self
+            unfold FunctionFreeConjunction.vars at subset
+            rw [List.mem_flatMap] at subset
+            rw [List.mem_flatMap]
+            rcases subset with ⟨a, a_mem, hd_mem⟩
+            exists trg.subs.apply_function_free_atom a
+            constructor
+            . apply List.mem_map_of_mem; exact a_mem
+            . simp only [GroundSubstitution.apply_function_free_atom]
+              unfold FunctionFreeAtom.variables at hd_mem
+              rw [List.mem_map]
+              exists VarOrConst.var hd
+              constructor
+              . apply VarOrConst.filterVars_occur_in_original_list; exact hd_mem
+              . simp [GroundSubstitution.apply_var_or_const]
+
+    apply this trg.rule.body.vars _ []
+    . apply List.getElem_mem
+    . simp
+    . simp
+    . simp
 
